\chapter{Progressions}
\begin{enumerate}
\item Given $t_n = 2n^2 + 1 \Rightarrow t_{n - 1} = 2(n - 1)^2 + 1$

  $\therefore d = t_n - t_{n - 1} = 4n - 2$, which is not constant. Hence, the sequence is not in A.P.
\item Given, $t_1 = 1, t_2 = 2$ and $t_{n+2} = t_n + t_{n + 1}$

  $\therefore t_3 = t_1 + t_2 = 3, t_4 = t_2 + t_3 = 5, t_5 = t_3 + t_4 = 8$.
\item Given $t_n = 3n + 5 \Rightarrow t_1 = 3\times1 + 5 = 8, t_2 = 3\times2 + 5 = 11, t_3 = 3\times3 + 5 = 14$. So the seuquence
  is $8, 11, 14, \ldots, 3n + 5$.
\item Given $t_n = 2n^2 + 3 \Rightarrow t_1 = 2\times1^2 + 3 = 5, t_2 = 2\times2^2 + 3 = 11, t_3 = 2\times3^2 + 5 = 23$. So the
  sequence is $5, 11, 23, \ldots, 2n^2 + 3$.
\item Given, $t_n = \frac{3n}{2n + 4}\Rightarrow t_1 = \frac{3\times1}{2\times1 + 4} = \frac{3}{6} = \frac{1}{2}, t_2 =
  \frac{3\times2}{2\times2 + 4} = \frac{6}{8} = \frac{3}{4}, t_3 = \frac{3\times3}{2\times3 + 4} = \frac{9}{10}$. So the
  sequence is $\frac{1}{2}, \frac{3}{4}, \frac{9}{10}, \cdots, \frac{3n}{2n + 4}$.
\item Given, $t_1 = 2, t_{n + 1} = \frac{2t_n + 1}{t_n + 3} \Rightarrow t_2 = \frac{2t_1 + 1}{t_1 + 3} = \frac{2\times1 + 1}{1 + 3}
  = \frac{3}{4}, t_3 = \frac{2t_2 + 1}{t_2 + 3} = \frac{2\times\tfrac{3}{4} + 1}{\tfrac{3}{4} + 3} = \frac{10}{15} = \frac{2}{3}$.
  So the sequence is $2, \frac{3}{4}, \frac{2}{3}, \cdots$.
\item Given, $t_n = 4n^2 + 1 \Rightarrow t_{n - 1} 4(n - 1)^2 + 1$

  $\therefore d = t_n - t_{n - 1} = 8n - 4$, which is not constant. Hence the sequence is not in A.P.
\item Given $t_n = 2an + b \Rightarrow t_{n - 1} = 2a(n - 1) + b$

  $\therefore d = t_n - t_{n - 1} = 2a$. which is a constant. Hence the sequence will be an A.P.
\item Given, $t_1 = 3, t_2 = 3, t_3 = 6$ and $t_{n + 2} = t_n + t_{n + 1}$

  $\therefore t_4 = t_2 + t_3 = 3 + 6 = 9$ and $t_5 = t_3 + t_4 = 6 + 9 = 15$.
\item $t_1 = 1 = a + b + c, t_2 = 5 = 4a + 2b + c$ and $t_3 = 11 = 9a + 3b + c$

  $\therefore t_2 - t_1 = 4 = 3a + b$ and $t_3 - t_2 = 6 = 5a + b$

  $\Rightarrow 2a = 2 \Rightarrow a = 1 \Rightarrow b = 1 \Rightarrow c = -1$

  $\Rightarrow t_{10} = 1\times10^2 + 1\times10 - 1 = 109$.
\item Difference between successive terms i.e. commond difference, $d = 12 - 9 = 15 - 12 = 18 - 15 = 3$ which is a constant, hence,
  the given sequence is an A.P.

  Here first term $t_1 = 9$ and $d = 3 \therefore t_{16} = 9 + (16 - 1)3 = 54$ and $t_n = 9 + (n - 1)3 = 3(n + 2)$.
\item $t_1 = \log a, t_2 = \log(ab) = \log a + \log b, t_3 = \log(ab^2) = \log a + 2\log b$

  $t_2 - t_1 = t_3 - t_2 = \log b$. Clearly, $t_1 = \log a, d = \log b$ which is constant so the sequence is an A.P.

  $\therefore t_n = \log a + (n - 1)\log b = \log(ab^{n - 1})$.
\item Given, $t_n = 5 - 6n \Rightarrow t_1 = 5 - 6 = -1$

  $S_n = \frac{n}{2}[t_1 + t_n] = n(2 - 3n)$.
\item $d = 7 - 3 = 11 -7 = 4, t_n = 407 = 3 + (n - 1)d \Rightarrow n = \frac{404}{4} + 1 = 102$.
\item Since $a, b, c, d, e$ are in A.P. $\therefore a + e = b + d = 2c = k$(say)

  $\therefore a - 4b + 6c - 4d + e = (a + e) - 4(b + d) + 3.2c = k - 4k + 3k = 0$.
\item Let $a$ be the first term and $d$ be the common difference of the given A.P.

  Given, $5t_5 = 8t_8 \Rightarrow 5a + 20d = 8a + 56d \Rightarrow 3a = -36d \Rightarrow a = -12d$

  $\Rightarrow t_{13} = a + 12d = 0$.
\item Let $n$th term be the smallest positive number. From the sequence we obtain that $t_1 = 25$ and $d = -2\frac{1}{4} = -\frac{9}{4}$.

  Then $t_n > 0 \Rightarrow 25 - (n - 1)\frac{9}{4} > 0\Rightarrow n < \frac{25\times4}{9} + 1 \Rightarrow n = 12$.
\item The given pay scale represents an A.P. with $t_1 = 700, d = 40$ and $t_n = 1500$.

  $\therefore t_n = t_1 + (n - 1)d \Rightarrow n = \frac{t_n - t_1}{d} + 1 = \frac{1500 - 700}{40} + 1 = 21$.

  Thus, the person will reach maximum payment in $21$ years.
\item Let $a$ be the first term and $d$ be the common difference of the A.P. According to the question,

  $t_7 = a + 6d = 34$ and $t_{13} = a + 12d = 64$

  Subtracting $6d = 30 \Rightarrow d = 5 \Rightarrow a = 4$. So the A.P. is $4, 9, 14, \ldots$.
\item If $55$ is the $n$th term then $n$ will have to be an integer. From the given sequence $a = 1, d = 3 - 1 = 5 - 3 = 2$.

  $55 = 1 + (n - 1)2 \Rightarrow n = 28$, which is an integer and hence, $55$ will be $28$th term of the A.P.
\item From the given sequence $a = 2000, d = 1995 - 2000 = 1990 - 1995 = -5$.

  Let $n$th term be first negative term, then, $a + (n - 1)d < 0 \Rightarrow 2000 -(n - 1)5 < 0$

  \Rightarrow $n > 401 \Rightarrow n = 402 \Rightarrow t_{402} = 2000 - (402 - 1)5 = -5$.
\item Common different of the sequence $2, 4, 6, 8, \ldots$ is $2$ and common difference of the seqquence $3, 6, 9, \ldots$ is $3$.

  Thus, common terms will have a common different which is L.C.M. of these two commond differences i.e. $6$.

  Last term of first sequence is $200$ and last term of second sequence is $240$. Clearly, last identical(common) number will be
  less than $200$. We also observe that $6$ is the first identical term. Let there be $n$ such terms. Then

  $6 + (n - 1)6 \leq 200 \Rightarrow n\leq \frac{194}{6} + 1 \Rightarrow n = 33$. Thus there will be $33$ identical terms in the two
  given A.P.
\item Clearly the first number of three digits divisible by $5$ is $100$; while the last such number is $995$. Since these numbers
  are all divisible by $5$ they will form an A.P. with common difference $5$.

  Clearly, $t_1 = 100, t_n = 995, d = 5$ and we have to find $n$.

  $t_n = 995 = 100 + (n - 1)5\Rightarrow n = 180$.
\item Given sequence is $4, 9, 14, \ldots$. So $a = 4, d = 9 - 4 = 14 - 9 = 5$. Let $105$ be $n$th term of this A.P. then $n$ has
  to be an integer for this assumption to be true.

  $105 = 4 + (n - 1)5 \Rightarrow n = \frac{106}{5}$ which is not an integer and therefore $105$ is not a term in the given A.P.
\item This problem is same as problem $21$ and has been left as an exercise.
\item This problem is same as problem $22$ and has been left as an exercise.
\item Let $a$ be the first term and $d$ be the common difference of the A.P. Given,

  $mt_m = nt_n \Rightarrow ma + (m - 1)md = na + (n - 1)nd \Rightarrow (m - n)a = (n^2 - n - m^2 + m)d$

  $\Rightarrow a = -(m + n - 1)d\,\therefore t_{m + n} = a + (m + n - 1)d = 0$.
\item Let $x$ be the first term and $y$ be the common difference of the A.P. Then,

  $a = x + (p - 1)y, b = x + (q - 1)y, c = x + (r - 1)y$

  We have to prove that $a(q - r) + b(r - p) + c(p - q) = 0$.

  Substituting the values of $a, b$ and $c$ in the above equation

  L.H.S. $= [x + (p - 1)y](q - r) + [x + (q - 1)y](r - p) + [x + (r - 1)y](p - q)$

  $= x(q - r + r - p + p - q) + y[(p - 1)(q - r) + (q - 1)(r - p) + (r - 1)(p - q)]$

  $= 0 =$ R.H.S.
\item First number after $100$ which is divisible by $7$ is $105$. The last number divisible by $7$ before $1000$ is $994$.

  Let $n$ be the numbers divisible by $7$ between $100$ and $1000$. Then $994 = 105 + (n - 1)7$

  $\Rightarrow n = 128$. Then no. of numbers not divisible by $7$ is $1000 - 100 - 128 = 772$.
\item Let $x$ be the first term and $y$ be the common difference of the A.P. Then,

  $a = x + (p - 1)y, b = x + (q - 1)y, c = x + (r - 1)y$

  We have to prove that $(a - b)r + (b - c)p + (c - a)q = 0$

  Substituting the values of $a, b$ and $c$ in the above equation

  L.H.S. $= (p - q)yr + (q - r)yp + (r - p)yq = 0 =$ R.H.S.
\item Let the numbers in A.P. be $a - d, a$ and $a + d$. Given their sum is $27$ and sum of squares is $293$.

  $\therefore a - d + a + a + d = 27 \Rightarrow a = 9$

  $\therefore (a - d)^2 + a^2 + (a + d)^2 = 293 \Rightarrow 3a^2 + 2d^2 = 293 \Rightarrow 3\times81 + 2d^2 = 293$

  $\Rightarrow 2d^2 = 50 \Rightarrow d = \pm5$

  So the numbers are $4, 9, 14$ or $14, 9, 4$.
\item Let the numbers in A.P. be $a - 3d, a - d, a + d, a + 3d$. Given their sum is $24$ and product is $945$.

  $\therefore a - 3d + a - d + a + d + a + 3d = 24 \Rightarrow 4a = 24 \Rightarrow a = 6$

  Also, $(a - 3d)(a - d)(a + d)(a + 3d) = 945 \Rightarrow (a^2 - 9d^2)(a^2 - d^2) = 945$

  $\Rightarrow a^4 - 10a^2d^2 + 9d^4 = 945 \Rightarrow 9d^4 - 360d^2 + 1296 - 945 = 0$

  $\Rightarrow 9d^4 - 360d^2 + 351 = 0 \Rightarrow d^4 - 40d^2 + 39 = 0$

  $\Rightarrow (d^2 - 1)(d^2 - 39) = 0$. Since the numbers are integers $\Rightarrow d^2 \neq 39$.

  $\Rightarrow d = \pm 1$. So the numbers are $3, 5, 7, 9$ or $9, 7, 5, 3$.
\item Let $a$ be the first term and $d$ be the common ratio of the A.P. Given,

  $t_p = a + (p - 1)d = q$ and $t_q = a + (q - 1)d = p$

  $\Rightarrow (p - q)d = q - p \Rightarrow d = -1 \Rightarrow a = p + q - 1$

  $\Rightarrow t_{p + q} = a + (p + q - 1)d = p + q - 1 - (p + q - 1) = 0$.
\item Let $a$ be the first term and $d$ be the common ratio of the A.P.

  $\Rightarrow t_m = a + (m - 1)d, t_{2n + m} = a + (2n + m - 1)d$

  $\Rightarrow t_m + t_{2n + m} = 2a + (2m + 2n - 2)d = 2[a + (m + n - 1)d] = 2t_{m + n}$
\item Let the three numbers be $a - d, a, a + d$. Given that their sum is $15$ and sum of their square is $83$.

  $\Rightarrow a - d + a + a + d = 15 \Rightarrow 3a = 15 \Rightarrow a = 5$

  $\Rightarrow (a - d)^2 + a^2 + (a + d)^2 = 83 \Rightarrow 3a^2 + 2d^2 = 83 \Rightarrow 3\times5^2 + 2d^2 = 83^2$

  $\Rightarrow d = \pm2$. So the numbers are $3, 5, 7$ or $7, 5, 3$.
\item This problem is similar to previous problem and has been left as an exercise.
\item Let the three numbers be $a - d, a, a + d$. Given their sum as $12$ and sum of cubes as $408$.

  $\therefore a - d + a + a + d = 12 \Rightarrow 3a = 12 \Rightarrow a = 4$

  $\therefore (a - d)^3 + a^3 + (a + d)^3 = 3a^3 + 6ad^2 = 408 \Rightarrow 24d^2 = 216 \Rightarrow d = \pm 3$

  Hence, the numbers are $1, 4, 7$ or $7, 4, 1$.
\item Let the numbers in A.P. be $a - 3d, a - d, a + d, a + 3d$. Given their sum is $24$ and product of first and
  fourth to product of second and third is $2:3$.

  $\therefore a - 3d + a - d + a + d + a + 3d = 20 \Rightarrow 4a = 20 \Rightarrow a = 5$

  $\therefore \frac{(a - 3d)(a + 3d)}{(a - d)(a + d)} = \frac{2}{3}$

  $\Rightarrow 3a^2 - 27d^2 = 2a^2 - 2d^2 \Rightarrow a^2 = 25d^2 \Rightarrow d = \pm1$.

  Therefore numbers are $2, 4, 6, 8$ or $8, 6, 4, 2$.
\item Let the three numbers be $a - d, a, a + d$. Given their sum is $-3$ and product is $8$.

  $\therefore a - d + a + a + d = -3 \Rightarrow 3a = -3 \Rightarrow a = -1$

  $\therefore (a - d).a.(a + d) = 8 \Rightarrow a^2 - d^2 = -8 \Rightarrow d = \pm3$

  Hence the numbers are $-4, -1, 2$ or $2, -1, -4$.
\item This problem is similar to problem 38 and has been left as an exercise.
\item Given $\frac{b + c - a}{a}, \frac{c + a - b}{b}, \frac{a + b - c}{c}$ are in A.P.

  Adding $2$ to each term will give us another A.P. [refer properties of A.P.]

  $\therefore \frac{a + b + c}{a}, \frac{a + b + c}{b}, \frac{a + b + c}{c}$ will be in A.P.

  Dividing each term with $a + b + c$ will yield another A.P.

  $\therefore \frac{1}{a}, \frac{1}{b}, \frac{1}{c}$ will be in A.P.
\item Given $a, b, c$ are in A.P.

  Dividing each term by $abc$ will yield another A.P.

  $\therefore \frac{1}{bc}, \frac{1}{ca}, \frac{1}{ab}$ will be in A.P.

  Multiplying each term with $abc + 1$ will yield another A.P.

  $\therefore a + \frac{1}{bc}, b + \frac{1}{ca}, c + \frac{1}{ab}$ will be in A.P.
\item Given $a, b, c$ are in A.P. $\therefore b - a = c - b$

  $\Rightarrow \frac{1}{b - a} = \frac{1}{c - b} \Rightarrow \frac{ab + bc + ca}{b - a} = \frac{ab + bc + ca}{c - b}$

  $\Rightarrow ab(b - a) + c(b^2 - a^2) = bc(c - a) + a(c^2 - b^2)$

  $\Rightarrow b^2a + b^2c - a^2b - a^2c = c^2a + c^2b - b^2c - b^2a \Rightarrow b^2(a + c) - a^2(b + c) = c^2(a + b) - b^2(c + a)$

  $\therefore a^2(b + c), b^2(c + a), c^2(a + b)$ are in A.P.
\item We will prove this in reverse. We assume that $\frac{1}{\sqrt{b} + \sqrt{c}}, \frac{1}{\sqrt{c} + \sqrt{a}},
  \frac{1}{\sqrt{a} + \sqrt{b}}$ are in A.P.

  $\Rightarrow \frac{1}{\sqrt{c} + \sqrt{a}} - \frac{1}{\sqrt{b} + \sqrt{c}} = \frac{1}{\sqrt{a} + \sqrt{b}} +
  \frac{1}{\sqrt{c} + \sqrt{a}}$

  $\Rightarrow \frac{2}{\sqrt{c} + \sqrt{a}} = \frac{1}{\sqrt{b} + \sqrt{c}} + \frac{1}{\sqrt{a} + \sqrt{b}}$

  $\Rightarrow \frac{2}{\sqrt{c} + \sqrt{a}} = \frac{\sqrt{a} + \sqrt{b} + \sqrt{b} + \sqrt{c}}{(\sqrt{b} + \sqrt{c})(\sqrt{a}
    + \sqrt{b})}$

  $\Rightarrow 2(\sqrt{b} + \sqrt{c})(\sqrt{a} + \sqrt{b}) = (\sqrt{c} + \sqrt{a})(\sqrt{a} + 2\sqrt{b} + \sqrt{c})$

  $\Rightarrow 2(\sqrt{ab} + b + \sqrt{ac} + \sqrt{bc}) = \sqrt{ac} + 2\sqrt{bc} + c + a + 2\sqrt{ab} + \sqrt{ac}$

  $\Rightarrow 2b = a + c$, which implies that $a, b, c$ are in A.P. So the reverse is also true.
\item Given $a, b, c$ are in A.P.

  Dividing each term by $abc$ will yield another A.P.

  $\Rightarrow \frac{1}{bc}, \frac{1}{ca}, \frac{1}{ab}$ will be in A.P.

  Multiplying each term with $ab + bc + ca$ will yield another A.P.

  $\Rightarrow \frac{ab + ca}{bc} + 1, \frac{ab + bc}{ca} + 1, \frac{bc + ca}{ab} + 1$ will be in A.P.

  Subtracting $1$ from each term yields desired terms in A.P.
\item We have to prove that $\frac{1}{b - c}, \frac{1}{c - a}, \frac{1}{a - b}$ are in A.P.

  i.e. $\frac{1}{c - a} - \frac{1}{b - c} = \frac{1}{a - b} - \frac{1}{c - a}$

  $\Rightarrow \frac{b -2c + a}{(c - a)(b - c)} = \frac{c - 2a + b}{(a - b)(c - a)}$

  $\Rightarrow (a + b - 2c)(a - b) = (b + c - 2a)(b - c)$

  Now, given that $(b - c)^2, (c - a)^2, (a - b)^2$ are in A.P.

  $\Rightarrow (c - a)^2 - (b - c)^2 = (a - b)^2 - (c - a)^2$

  $\Rightarrow (b - a)(2c - a - b) = (c - b)(2a - b - c)$

  Thus, we have proven the desierd result.
\item Given $a, b, c$ are in A.P.

  Subtracting $a, b, c$ from each term will yield another A.P.

  $\Rightarrow -(b + c), -(c + a), -(a + b)$ will be in A.P.

  Multiplying each term with $-1$ will yield the desired A.P.
\item We have to prove that $\frac{1}{b + c}, \frac{1}{c + a}, \frac{1}{a + b}$ are in A.P.

  i.e. $\frac{1}{c + a} - \frac{1}{b + c} = \frac{1}{a + b} - \frac{1}{c + a}$

  $\Rightarrow \frac{b - a}{(b + c)} = \frac{c - b}{(a + b)}$

  $\Rightarrow b^2 - a^2 = c^2 - b^2 \Rightarrow a^2, b^2, c^2$ are in A.P.

  Thus, we have proven the desired result in reverse.
\item Given that $a, b, c$ are in A.P. $\Rightarrow b - a = c - b = k$ (say)

  $\Rightarrow c - a = 2k \Rightarrow 2(a - b) = a - c = 2(b - c) = -2k$.
\item Given that $a, b, c$ are in A.P. Let $b = a + d \Rightarrow c = a + 2d$

  Now, $(a - c)^2 = 4d^2, 4(b^2 - ac) = 4[(a + d)^2 - a(a + 2d)] = 4d^2$

  $\Rightarrow (a - c)^2 = 4(b^2 - ac)$
\item Let $n = 2m + 1$ where $m\in N. \Rightarrow S_1 = \frac{n}{2}[t_1 + t_n]$ where $d$ is the commond difference.

  For $S_2$ the no. of terms will be $m. \Rightarrow S_2 = \frac{m}{2}[t_2 + t_{n - 1}]$

  We know that $t_1 + t_n = t_2 + t_{n - 1}$

  $\therefore \frac{S_1}{S_2} = \frac{n}{m} = \frac{n}{\tfrac{n - 1}{2}} = \frac{2n}{n - 1}$.
\item The degree is the highest power of $x$ which will be $1 + 6 + 11 + \cdots + 101$.

  Clearly, the above sequence is an A.P. having first term $1$, common difference $5$ and last term as $101$.

  $n = \frac{t_n - t_1}{d} + 1 = \frac{101 - 1}{5} + 1 = 21$.

  $\Rightarrow S = \frac{21}{2}[t_1 + t_n] = \frac{21}{2}[1 + 101] = 21\times 51 = 1071$

  Therefore, the degree of the polynomial will be $1071$.
\item Consider an A.P. with first term as $a$, commond difference as $d$ and no. of terms as $n$. Then sum is given by

  $S = \frac{n}{2}[2a + (n - 1)]d = \frac{n^2d^2}{2} + \frac{(2a - d)n}{2}$

  which is of the form $An^2 + Bn$ where $A = \frac{d^2}{2}$ and $B = \frac{2a - d}{2}$.
\item Let the common difference of the A.P. be $d$.

  L.H.S. $= a_1^2 - a_2^2 + a_3^2 - a)4^2 + \cdots + a_{2n - 1}^2 -a_{2n}^2$

  $= (a_1 - a_2)(a_1 + a_2) + (a_3 - a_4)(a_3 + a_4) + \cdots + (a_{2n - 1} - a_{2n})(a_{2n - 1} + a_{2n})$

  $= -d(a_1 + a_2 + a_3 + a_4 + \cdots + a_{2n - 1} + a_{2n})$

  $= -\frac{2nd}{2}[a_1 + a_{2n}]$

  $= \frac{n}{2n - 1}(a_1^2 - a_{2n}^2)\left[\because d = \frac{a_{2n} - a_1}{2n - 1}\right]$
\item We know that sum of equidistant terms from start and end of an A.P. is equal.

  $\therefore a_1 + a_{24} = a_5 + a_{20} = a_{10} + a_{15} = k$ (say)

  $\therefore a_1 + a_5 + a_{10} + a_{15} + a_{24} = 3k = 225 \Rightarrow k = 75$

  Sum of first $24$ terms $S = a_1 + a_2 + \cdots + a_{24} = \frac{24}{2}[a_1 + a_{24}] = 12\times75 = 600$.
\item Let $a$ be the first term and $d$ be the common difference. Also let $S_1$ denote the sum of first $3n$ terms and $S_2$
  denote the sum of next $n$ terms.

  $S_1 = \frac{3n}{2}[2a + (3n - 1)d], S_2 = \frac{n}{2}[2a + 6nd + (n - 1)d][\because t_{3n+1} = a + 3nd]$

  Given, $S_1 = S_2 \Rightarrow \frac{3n}{2}[2a + (3n - 1)d] = \frac{n}{2}[2a + 6nd + (n - 1)d]$

  $\Rightarrow 6a + (9n - 3)d = 2a + (7n - 1)d \Rightarrow 2a + (n - 2)d = 0$

  Let $S_3$ be sum of first $2n$ terms and $S_4$ be sum of next $2n$ terms, then

  $\frac{S_3}{S_4} = \frac{\tfrac{2n}{2}[2a + (2n - 1)d]}{\tfrac{2n}{2}[2a + 4nd + (2n - 1)]d}$

  $\Rightarrow = \frac{nd}{5nd} = \frac{1}{5}[\because 2a + (n - 1)d = 0xs]$
\item Given $S_n = 5n^2 + 3n \Rightarrow t_n = S_n - S_{n - 1} = 5n^2 + 3n - 5(n - 1)^2 - 3(n - 1)$

  $= 10n - 5 + 3 = 10n - 2 \Rightarrow d = t_n - t_{n - 1} = 10n - 2 - 10(n - 1) + 2 = 10$,

  Since common difference is a constant the series is in A.P.
\item Common difference of the series $d = (a^2 + b^2) - (a + b)^2 = (a - b)^2 - (a^2 + b^2) = -2ab$

  $S = \frac{n}{2}[2(a + b)^2 - (n - 1)2ab] = \frac{n}{2}[2a^2 + 2b^2 - 2(n + 1)ab]$

  $= n[a^2 + b62 - (n + 1)ab]$.
\item There will be two cases. First $n$ being odd and second $n$ being even.

  {\bf Case I:} When $n$ is odd i.e. $n = 2m + 1$, where $m = 0, 1, 2, \ldots$

  $S = 1 + 5 + 9 + \cdots$ up to $m + 1$ terms $- 3 - 7 - 11$ up to $m$ terms

  $= \frac{m + 1}{2}[2 + 4m] - \frac{m}{2}[6 + 4m - 4] = (m + 1)(1 + 2m) - m(2m + 1)$

  $= 2m^2 + 3m + 1 - 2m^2 - m = 2m + 1 = n$.

  {\bf Case II:} When $n$ is even i.e. $n = 2m$, where $m =1, 2, 3, \ldots$

  $S = 1 + 5 + 9 + \cdots$ up to $m$ terms $- 3 - 7 - 11$ up to $m$ terms

  $= \frac{m}{2}[2 + 4m - 4] - \frac{m}{2}[6 + 4m - 4] = -2m = -n$.
\item Let there be $n$ sides of the polygon. From geometry, we know that sum of angles of the polygon $= (n - 2)180^\circ$

  From the formula for sum of an A.P. $S = \frac{n}{2}[2\times120^\circ + (n - 1)5^\circ] = (n - 2)180^\circ$

  $\frac{n}[240^\circ + (n - 1)5^\circ] = (n - 2)360^\circ\Rightarrow n[48^\circ + (n - 1)] = (n - 2)72^circ$

  $\Rightarrow n^2 - 25n + 144 = 0 \Rightarrow n = 9, 16$
\item To water first tree the gardener will have to travel $10$ m. To water second tree he will
  have tp travel back $10$ m to well and then $15$ m to the tree i.e. $25$ m. Similarly, for third tree he will
  have to travel $15$ m to well and $20$ m i.e a total of $35$ m.

  Thus, total distance travelled will be $10 + 25 + 35 + \cdots$

  Clearly, $25$ will be the first term of the A.P. and there will be $24$ such terms because distance travelled
  for first tree is noty part of the A.P. Note that common difference would be $10$.

  Total distance travelled $= 10 + \frac{24}{2}[2\times25 + (24 - 1)10] = 10 + 3360 = 3370$ m.
\item Let $d$ be the common difference. Given $S_p = 0 \Rightarrow \frac{p}{2}[2a + (p - 1)d] = 0$

  $\Rightarrow 2a + (p - 1)d = 0 \Rightarrow d = \frac{2a}{1 - p}$

  $p + 1$th term $t_{p + 1} = a + pd$, so the sum of next $q$ terms $S = \frac{q}{2}[2a + 2pd + (q - 1)d]$

  $= \frac{q}{2}[2a + (2p + q - 1)d] = \frac{q}{2}\left[2a + (2p + q - 1).\frac{2a}{1 - p}\right]$

  $= \frac{q}{2}\left[\frac{2a.(p + q)}{1 - p}\right] = -\frac{a(p + q)}{p - 1}q$.
\item Sum of first $p$ terms, $S_p = \frac{p}{2}[2a + (p - 1)d]$; sum of first $q$ terms $S_q = \frac{q}{2}[2a + (q - 1)d]$

  $2ap + (p^2 - p)d = 2aq + (q^2 - q)d \Rightarrow 2a(p - q) = (q^2 - p^2 + p - q)d$

  $2a = (1 - p - q)d$

  Sum of $(p + q)$ terms, $S_{p + q} = \frac{p + q}{2}[2a + (p + q - 1)d] = \frac{p + q}{2}[(1 - p - q)d + (p + q - 1)d] = 0$.
\item Sum of latter half of $2n$ terms means $n + 1$th term to $2n$th term. $t_{n + 1} = a + nd$ and $t_{2n} = a + (2n - 1)d$
  where $a$ and $d$ are the first term and common difference respectively.

  Sum of latter half of terms, $S = \frac{n}{2}[t_{n + 1} + t_{2n}] = \frac{n}{2}[2a + (3n - 1)d]$

  Sum of first $3n$ terms, $S_{3n} = \frac{3n}{2}[2a + (3n - 1)d]$

  Clearly, $S/S_{3n} = 1:3$.
\item Let $S_r$ be the $r$th A.P. whose first term is $r$ and common difference is also $r$.

  $S_r = \frac{n}{2}[2r + (n - 1)r] = \frac{n}{2}[(n + 1)r] = \frac{n(n + 1)r}{2}$

  $S_1 + S_2 + S_3 + \cdots + S_p = \displaystyle\sum_{r=1}^pS_r$

  $= \frac{n(n + 1)}{2}\displaystyle\sum_{r = 1}^pr = \frac{np}{4}(n + 1)(p + 1)\left[\because\displaystyle\sum_{i=1}^ni =
  \frac{n(n + 1)}{2}\right]$.
\item Let $x$ be the first term and $y$ be the common difference of the A.P.

  Then, according to the question $a = \frac{p}{2}[2x + (p - 1)y], b = \frac{q}{2}[2x + (q - 1)y], c = \frac{r}{2}[2x + (r - 1)y]$

  We have to prove that $\frac{a}{p}(q - r) + \frac{b}{q}(r - p) + \frac{c}{r}(p - q) = 0$

  L.H.S. $= x(q - r + r - p + p - q) + \frac{y}{2}[(p - 1)(q - r) + (q - 1)(r - p) + (r - 1)(p - q)]$

  $= 0$.
\item Let $a$ be the first term and $d$ be the common difference of the A.P.

  Given, $S_m = \frac{1}{2}S_{m + n}\Rightarrow \frac{m}{2}[2a + (m - 1)d] = \frac{1}{2}.\frac{m + n}{2}[2a + (m + n - 1)d]$

  Let $2a + (m - 1)d = x$, then the above equation can be written as

  $mx = \frac{m + n}{2}[x + nd] \Rightarrow 2mx = (m + n)[x + nd]\Rightarrow mx = n(x + nd) + mnd$

  $\Rightarrow (m - n)x = (m + n)nd$

  Similarly, $(m - p)x = (m + p)pd$

  Dividing, we get

  $(m - n)(m + p)p = (m + n)(m - p)n$

  Dividing both sides with $mnp$ we arrive at the desired result.
\item Let $a$ be the first term and $d$ be the common difference of the A.P. For odd terms, the no. of terms will be $n + 1$, first
  term will be $a$ and common difference will be $2d$.

  $\therefore S_{odd} = \frac{n + 1}{2}[2a + 2nd]$

  For even terms, the no. of terms will be $n$, first term will be $a + d$ and common difference will be $2d$.

  $\therefore S_{even} = \frac{n}{2}[2a + 2d + 2(n - 1)d] = \frac{n}{2}[2a + 2nd]$

  $\therefore \frac{S_{odd}}{S_{even}} = \frac{n + 1}{n}$.
\item Let $a_1$ and $a_2$ be the first terms and $d_1$ and $d_2$ be the common differences of the two series in A.P.

  Given, $\frac{\tfrac{n}{2}[2a_1 + (n - 1)d_1]}{\tfrac{n}{2}[2a_2 + (n - 1)d_2]} = \frac{3n - 12}{5n + 21}$

  $\Rightarrow \frac{2a_1 + (n - 1)d_1}{2a_2 + (n - 1)d_2} = \frac{3n - 13}{5n + 21}$

  We need to find ratio of the $24$th terms i.e. $\frac{a_1 + 23d_1}{a_2 + 23d_2} = \frac{2a_1 + 46d_1}{2a_2 + 46d_2}$

  Putting $n = 47$ in the ratio of sums, we have

  $\frac{2a_1 + 46d_1}{2a_2 + 46d_2} = \frac{3\times 47 - 13}{5\times47 + 21} = \frac{1}{2}$
\item Let $a$ be the first term and $d$ be the common difference of the A.P.

  Given, $t_m = a + (m - 1)d = \frac{1}{n},\,t_n = a + (n - 1)d = \frac{1}{m}$

  Subtracting, we get $(m - n)d = \frac{m - n}{mn} \Rightarrow d = \frac{1}{mn} \Rightarrow a = \frac{1}{mn}$

  $\therefore S_{mn} = \frac{mn}{2}\left[\frac{2}{mn} + \frac{mn - 1}{mn}\right] = \frac{mn + 1}{2}$.
\item Let $a$ be the first term and $d$ be the common difference of the A.P.

  Given, $S_m = n = \frac{m}{2}[2a + (m - 1)d] \Rightarrow 2a + (m - 1)d = \frac{2n}{m}$

  and $S_n = m = \frac{n}{2}[2a + (n - 1)d] \Rightarrow 2a + (n - 1)d = \frac{2m}{n}$

  $\Rightarrow d = -\frac{2(m + n)}{mn}\Rightarrow a = \frac{m^2 + n^2 + mn - m - n}{mn}$

  $\Rightarrow S_{m + n} = \frac{m + n}{2}[2a + (m + n - 1)d] = -(m + n)$.
\item Let $a$ be the first term and $d$ be the common difference of the A.P.

  $\therefore S = \frac{2n + 1}{2}[2a + 2nd]$

  For $S_1$ first term would be $a$, common difference would be $2d$ and no. of terms would be $n + 1$.

  $\therefore S_1 = \frac{n + 1}{2}[2a + 2nd]$

  $\therefore \frac{S}{S_1} = \frac{2n + 1}{n +1}$.
\item Let $d$ be the common difference, then $b = a + 2d \Rightarrow d = \frac{b - a}{2}$

  $c = a + (n - 1)d \Rightarrow n - 1 = \frac{c - a}{d} = \frac{2(c - a)}{b - a}$

  $\Rightarrow n = \frac{2(c - a)}{b - a} + 1$

  $\therefore S = \frac{n}{2}[2a + (n - 1)d] = \frac{1}{2}\left[\frac{2(c - a)}{b - a} + 1\right]\left[2a + \frac{2(c - a)}{b -
    a}.\frac{b - a}{2}\right]$

  $= \frac{c + a}{2} + \frac{c^2 - a^2}{b - a}$.
\item Let $a_1, a_2$ be the first terms and $d_1, d_2$ be the common differences of the two series in A.P.

  According to the question $\frac{2a_1 + (n - 1)a_1}{2a_2 + (n - 1)d_2} = \frac{3n + 8}{7n + 15}$.

  We have to find ratio of $12$th terms i.e. $\frac{a_1 + 11d_1}{a_2 + 11d_2} = \frac{2a_1 + 22d_1}{2a_2 + 22d_2}$

  Putting $n = 23$ in previous equation, we get

  $\frac{2a_1 + 22d_1}{2a_2 + 22d_2} = \frac{77}{176} = \frac{7}{16}$.
\item Let $a$ be the first term and $d$ be the common difference of the A.P.

  Given, $\frac{S_m}{S_n} = \frac{\tfrac{m}{2}[2a + (m - 1)d]}{\tfrac{n}{2}[2a + (n - 1)d]} = \frac{m^2}{n^2}$

  $\Rightarrow \frac{2a + (m - 1)d}{2a + (n - 1)d} = \frac{m}{n}$

  $\Rightarrow 2a(n - m) + [(m - 1)n - (n - 1)m]d = 0 \Rightarrow a = \frac{d}{2}$

  We have to find $\frac{t_m}{t_n} = \frac{a + (m - 1)d}{a + (n - 1)d} = \frac{2m - 1}{2n - 1}$
\item Let $n$ be the no. of terms. Clearly, common ratio $r = \frac{20}{5} = \frac{80}{20} = 4$

  Then $t_n = 5120 = 5.r^{n - 1} \Rightarrow 4^{n - 1} = 1024 = 4^5 \Rightarrow n = 6$.
\item Let $n$ be the no. of terms. Clearly, common ratio $r = \frac{0.06}{0.03} = \frac{0.12}{0.06} = 2$

  Then $t_n = 3.84 = 0.03r^{n - 1} \Rightarrow 2^{n - 1} = 128 \Rightarrow n = 8$.
\item From the question we deduce that it is a G.P. with $a = 1, r = 2, n = 20$. We have to find $t_{20}$.

  $t_{20} = 1.2^{20 - 1} = 524288$.
\item This is a G.P. with $a = 20000, r = 1.02, n = 11$. We have to find $t_{11}$.

  $t_{11} = 20000\times(1.02)^{11 - 1} = 24380$.
\item Given, $S_n = 2^n - 1 \Rightarrow t_n = S_n - S_{n - 1} = 2^n - 1 - (2^{n - 1} - 1) = 2^{n - 1}$

  $r = \frac{t_n}{t_{n - 1}} = \frac{2^{n - 1}}{2^{n - 2}} = 2$, which is a constant and hence the sequence is in G.P.
\item Let the first term of the G.P. be $a$ and common ratio is $r$.

  Then $t_2 = ar = 24$ and $t_5 = ar^4 = 81$, Dividing, we have $r^3 = \frac{81}{24} = \frac{27}{8}$

  $\Rightarrow r = \frac{3}{2} \Rightarrow a = 16$.

  Hence the G.P. is $16, 24, 36, 54, 81, \ldots$.
\item Let the first term of the G.P. be $a$ and common ratio is $r$.

  Given $t_7 = 8t_4 \Rightarrow ar^6 = 8ar^3 \Rightarrow r = 2$. Also given, $t_5 = 48 \Rightarrow ar^4 = 48$

  $\Rightarrow a = 3$. Hence, the G.P. is $3, 6, 12, 24, \ldots$.
\item Let the first term of the G.P. be $a$ and common ratio is $r$.

  Given, $t_5 = ar^4 = 48$ and $t_8 = ar^7 = 384 \Rightarrow r^3 = 8 \Rightarrow r = 2$

  $\Rightarrow a = 3$. Hence, the G.P. is $3, 6, 12, 24, \ldots$.
\item Let the first term of the G.P. be $a$ and common ratio is $r$.

  Given $t_6 = ar^5 = \frac{1}{16}$ and $t_{10} = ar^9 = \frac{1}{256} \Rightarrow r = \pm\frac{1}{2}$

  $\Rightarrow a = \pm 2$. Hence the G.P. is $2, 1, \frac{1}{2}, \ldots$ or $-2, 1, -\frac{1}{2}, \ldots$.
\item Let the first term of the G.P. be $x$ and common ratio is $y$. Then

  $a = xy^{p - 1}, b = xy^{q - 1},  c = xy^{r - 1}$

  Taking $\log$ of both sides for these three terms

  $\log a = \log x + (p - 1)\log y, \log b = \log x + (q - 1)\log y, \log c = \log x + (r - 1)\log y$

  Clearly, $(q - r)\log a + (r - p)\log b + (p - q)\log r = 0$.
\item Let the first term of the G.P. be $x$ and common ratio is $r$.

  Given, $t_{p + q} = a = xr^{p + q - 1}$ and $t_{p - q} = b = xr^{p - q - 1}$

  Multiplying the two terms, we have

  $x^2r^{2p - 2} = (xr^{p - 1})^2 = t_p^2 = ab \Rightarrow t_p = \sqrt{ab}$.
\item Let $a$ be the first term and $b$ be the common ratio. Then,

  $x = ab^{p - 1}, y = ab^{q - 1}, z = ab^{r -1}$

  We have to prove that $x^{q - r}.y^{r - p}.z^{p - q} = 1$

  L.H.S. $= (ab^{p - 1})^{q - r}.(ab^{q - 1})^{r - p}.(ab^{r - 1})^{p - q}$

  $= a^{(q - r + r - p + p - q)}b^{[(p - 1)(q - r) + (q - 1)(r - p) + (r - 1)(p - q)]}$

  $= a^0b^0 = 1 =$ R.H.S.
\item Let $r$ be the common ratio and first term is given as $1$.

  $t_3 + t_5 = 90 \Rightarrow r^4 + r^2 = 90 \Rightarrow r^2 = 9 \Rightarrow r = pm 3$.

  $r^2$ cannot be $-10$ as that would mean that it is an imaginary number.
\item Let $a$ be the first term and $r$ be the common ratio of the G.P.

  Gibem $t_5 = ar^4 = 2$ and we have to find the product of the first nine terms. Let the required product be $S$.

  $S = a.ar.ar^2.\ldots.ar^8 = a^9r^{1 + 2 + \cdots + 8} = a^9r^{\tfrac{8.9}{2}} = a^9r^{36} = (ar^4)^9 = 2^9 = 512$.
\item Let $a$ be the first term, $r$ be the common ratio and $n$ be the number of terms.

  Given, $t_4 = ar^3 = 10, t_7 = ar^6 = 80, t_n = ar^{n - 1} = 2560$

  $\therefore \frac{t_7}{t_4} = r^3 = 8 \Rightarrow r = 2 \Rightarrow a = \frac{10}{8}$

  $\Rightarrow \frac{10}{8}2^{n- 1} = 2560 \Rightarrow 2^{n - 1} = 2048 \Rightarrow n = 12$.
\item Let the three numbers in G.P. be $a, ar, ar^2$. According to question, on doubling $ar$ the numbers form an A.P.

  $\Rightarrow 2ar - a = ar^2 - 2ar \Rightarrow r^2 - 4r + 1 = 0 \Rightarrow r = \frac{4\pm\sqrt{12}}{2} = 2\pm\sqrt{3}$.
\item Given, $p, q, r$ are in A.P. i.e. $q - p = r - q$.

  Let $x$ be the first term and $y$ be the common ratio of the G.P. We have to prove that $t_p, t_q, t_r$ are in G.P.

  $\Rightarrow \frac{t_q}{t_p} = \frac{t_r}{t_q} \Rightarrow \frac{xy^{q - 1}}{xy ^{p - 1}} = \frac{xy^{r - 1}}{xy^{q - 1}}$

  $\Rightarrow y^{q - p} = y^{r - q}$ which is true from the condition for A.P.
\item Let $r$ be the common ratio of the G.P. Then, $b = ar, c = ar^2, d = ar^3$

  L.H.S. $= (a.ar + ar.ar^2 + ar^2.ar^3)^2 = a^4r^2(1 + r^2 + r^4)^2$

  R.H.S. $= (a^2 + a^2r^2 + a^2r^4)(a^2r^2 + a^2r^4 + a^2r^6) = a^2(1 + r^2 + r^4).a^2r^2(1 + r^2 + r^4)$

  $= a^2r^4(1 + r^2 + r^4)^2 =$ L.H.S.
\item Given $a, b, c$ are in A.P. $\Rightarrow 2b = a + c$

  If we increase $a$ by $1$ then they are in G.P. $\Rightarrow b^2 = (a + 1)c \Rightarrow b^2 = (a + 1)(2b - a)$

  $\Rightarrow b^2 = 2ab - a^2 + 2b - a \Rightarrow (a - b)^2 = 2b - a$

  If we increase $c$ by $2$ then again they are in G. P $\Rightarrow b^2 = a(c + 2) = a(2b - a + 2)$

  $\Rightarrow b^2 = 2ab - a^2 + 2a \Rightarrow (a - b)^2 = 2a \Rightarrow 2b - a = 2a \Rightarrow 2b = 3a$

  $\Rightarrow \left(a - \frac{3a}{2}\right)^2 = 2a \Rightarrow a = 8 \Rightarrow b = 12 \Rightarrow c = 16$.
\item Let the three numbers in G.P. be $\frac{a}{r}, a, ar$. Then,

  $\frac{a}{r} + a + ar = 70$ and $10a = \frac{4a}{r} + 4ar \Rightarrow \frac{10a}{4} = \frac{a}{r} + ar$

  $\Rightarrow \frac{10a}{4} + a = 70 \Rightarrow a = 20$

  $\Rightarrow \frac{20}{r} + 20r = 50 \Rightarrow r = 2, \frac{1}{2}$

  So the numbers are $10, 20, 40$ or $40, 20, 10$.
\item Let the three numbers in G.P. be $\frac{a}{r}, a, ar$. Given that product of these numbers is $216$.

  $\Rightarrow \frac{a}{r}.a.ar = 216 \Rightarrow a^3 = 216 \Rightarrow a = 6$

  Also, given that their sum is $19 \Rightarrow \frac{6}{r} + 6 + 6r = 19$

  $\Rightarrow 6r^2 - 13r + 6 = 0 \Rightarrow r = \frac{2}{3}, \frac{3}{2}$.

  So the numbers are $9, 6, 4$ or $4, 6, 9$.
\item Let the number be $100a + 10ar + ar^2$.

  According to question $a + ar^2 = 2ar + 1$ and $a + ar = \frac{2}{3}(ar + ar^2)$

  $\Rightarrow a(r - 1)^2 = 1$ and $3 + 3r = 2r + 2r^2 \Rightarrow r = -1, \frac{3}{2}$

  If $r = -1, a = \frac{1}{4}$, but $a$ cannot be a fraction.

  If $r = \frac{3}{2} \Rightarrow a = 4$ and the number is $469$.
\item Given that three of four numbers are in A.P. and so we choose them as $a - d, a, a + d$. Also, since first number is same as
  first so the numbers are $a + d, a - d, a, a + d$. The first three are in G.P. Given $d = 6$

  $\therefore (a - d)^2 = a(a + d)\Rightarrow (a - 6)^2 = a(a + 6) \Rightarrow 18a = 36 \Rightarrow a = 2$.

  So the numbers are $8, -4, 2, 8$.
\item Let the three numbers are $a, ar, ar^2$. The sum is given as $21 \Rightarrow a + ar + ar^2 = 21$.

  Also, sum of squares is given as $189 \Rightarrow a^2 + a^2r^2 + a^2r^4 = 189$

  $\Rightarrow \frac{441(1 + r^2 + r^4)}{(1 + r + r^2)^2} = 189$

  $\Rightarrow 7(1 + 2r^2 + r^4 - r^2) = 3(r + r + r^2)^2 \Rightarrow 7(1 - r + r^2) - 3(1 + r + r^2)$

  $\Rightarrow 2r^2 - 5r + 2 = 0 \Rightarrow r = 2, \frac{1}{2}$

  When $r = 2, a = 3$ and so the numbers are $3, 6, 12$.

  When $r = \frac{1}{2}, a = 12$ and so the numbers are $12, 6, 3$.
\item Let the terms in G.P. be $\frac{a}{r}, a, ar$. Given that the product of these is $-64$.

  $\therefore \frac{a}{r}.a.ar = -64 \Rightarrow a^3 = -64 \Rightarrow a = -4$.

  Also given that the first term is four times the third. $\Rightarrow \frac{a}{r} = 4.ar \Rightarrow r^2 = \frac{1}{4} \Rightarrow r = \pm\frac{1}{2}$.

  If $r = \frac{1}{2},$ the terms will be $-8, -4, -2$. If $r = -\frac{1}{2}$, the terms will be $8, -4, 2$.
\item Let the numbers be $a - d, a, a + d$. Given that sum is $15. \Rightarrow a - d + a + a + d = 15 \Rightarrow a = 5$.

  Also given that if $1, 4, 19$ are added to them then they are in G.P.

  $\Rightarrow (5 + 4)^2 = (5 - d + 1)(5 + d + 19) \Rightarrow 81 = (6 - d)(24 + d)$

  $\Rightarrow d^2 + 18d - 63 = 0 \Rightarrow d = -21, 3$.

  If $d = -15$, the numbers will be $26, 5, -16$ and if $d = 3$ the numbers will be $2, 5, 8$.
\end{enumerate}
